examples/Weather.v
@@ -1,6 +1,6 @@
 Require Import AutoDB.
 
-Definition MEASUREMENT := "MEASUREMENT".
+Definition VALUE := "VALUE".
 Definition MEASUREMENT_TYPE := "MEASUREMENT_TYPE".
 Definition TIME := "TIME".
 Definition CELL_ID := "CELL_ID".
@@ -32,7 +32,7 @@ Definition WeatherSchema :=
               where attributes [STATE] depend on [AREA_CODE]; (* second clause? *)
       relation MEASUREMENTS has
               schema <CELL_ID :: nat,
-                      MEASUREMENT :: Z,
+                      VALUE :: Z,
                       MEASUREMENT_TYPE :: MeasurementType,
                       DAY :: nat,
                       TIME :: nat> ]
@@ -46,7 +46,7 @@ Definition WeatherSig : ADTSig :=
       "AddMeasurement" : rep × (WeatherSchema#MEASUREMENTS) → rep × bool,
       "CountCells"     : rep × AreaCode                        → rep × nat,
 (*      "CellIsActive"   : rep × nat                          → rep × bool, *)
-      "LocalCount"       : rep × (AreaCode * MeasurementType)    → rep × nat
+      "LocalMax"       : rep × (AreaCode * MeasurementType)    → rep × option Z
     }.
 
 Definition WeatherSpec : ADT WeatherSig :=
@@ -64,12 +64,12 @@ Definition WeatherSpec : ADT WeatherSig :=
              Where (area = cell!AREA_CODE)
              Return 1),
 
-     query "LocalCount" (params: AreaCode * MeasurementType) : nat :=
-        Count (For (cell in CELLS) (measurement in MEASUREMENTS)
-               Where (cell!AREA_CODE = fst params)
-               Where (measurement!MEASUREMENT_TYPE = snd params)
-               Where (cell!CELL_ID = measurement!CELL_ID)
-               Return 1)
+     query "LocalMax" (params: AreaCode * MeasurementType) : option Z :=
+        MaxZ (For (cell in CELLS) (measurement in MEASUREMENTS)
+              Where (cell!AREA_CODE = fst params)
+              Where (measurement!MEASUREMENT_TYPE = snd params)
+              Where (cell!CELL_ID = measurement!CELL_ID)
+              Return measurement!VALUE)
 }.
 
 Definition CellHeading := GetHeading WeatherSchema CELLS.
@@ -94,165 +94,6 @@ Definition Weather_AbsR
 Definition WeatherStation :
   Sharpened WeatherSpec.
 Proof.
-  Print Ltac plan. match goal with
-  | |- Sharpened ?spec =>
-        unfolder spec ltac:(fun spec' => change spec with spec')
-  end. start_honing_QueryStructure. hone_representation Weather_AbsR.
-
-  hone method "LocalCount".
-  Print Ltac observer.
-  Print Ltac observer'.
-
-  observer.
-  startMethod Weather_AbsR. 
-  concretize.
-  asPerm .
-  asPerm_indep.
-  asPerm_indep.
-  asPerm_indep.
-  asPerm_indep.
-  asPerm_indep.
-  Unset Ltac Debug.
-  asPerm_dep (CellsStorage, MeasurementsStorage).
-
-  asPerm_indep.
-  asPerm_dep (CellsStorage, MeasurementsStorage).
-
-  asPerm_indep.
-
-  match goal with
-    | [ |- _ ] =>
-                 setoid_rewrite filter_join_lists; simp
-  end.
-
-  match goal with
-    | [ |- context[filter _ (Join_Lists ?ls1 (filter ?f ?ls2))] ] =>
-      setoid_rewrite (swap_joins ls1 (filter f ls2)); trickle_swap; simp
-  end.
-  asPerm_indep.
-  repeat asPerm_indep.
-  asPerm Weather_AbsR.
-  asPerm_indep.
-  asPerm_indep.
-  Print Ltac asPerm_indep.
-  Check filter_join_lists.
-  match goal with
-  | |- context [filter ?F (Join_Lists _ _)] => pose F
-  end.
-
-  honeOne.
-  hone method "CountCells".
-  observer.
-
-  hone method "AddCell".
-  mutator.
-
-  hone method "AddMeasurement".
-  mutator. (* Badly needs a second index on CellIDs *)
-
-  hone method "LocalCount".
-  Print Ltac observer.
-  Print Ltac observer'.
-
-  startMethod Weather_AbsR. 
-  concretize.
-  Print Ltac asPerm_indep.
-  Check filter_join_lists.
-  match goal with
-  | |- context [filter ?F (Join_Lists _ _)] => pose F
-  end.
-
-Ltac getFst2 F k :=
-  match type of F with
-  | ?A * ?B -> ?C =>
-    let G := fresh "G" in let p := fresh "p" in let H := fresh "H" in
-    evar (G : A -> C); assert (H : forall p, F p = G (fst p)) by (subst G; intro p;
-      pattern (fst p);
-      match goal with
-      | [ |- (fun t => @?f t = @?g t) _ ] => equate g f; reflexivity
-      end); clear H;
-    let G' := eval unfold G in G in clear G; k G'
-  end.
-
-  Unset Ltac Debug.
-getFst2 (fun a: (@Tuple CellHeading) * (@Tuple MeasurementsHeading) => ?[eq_nat_dec (fst a)!AREA_CODE (fst n)]) ltac:(fun f => rewrite (filter_join_fst f)). getSnd F ltac:(fun f => rewrite (filter_join_snd f))
-
-  Print Ltac asPerm'.
-  asPerm storages.
-  commit. 
-  choose_db Weather_AbsR.
-  finish honing
-
-  observer' Weather_AbsR (CellsStorage, MeasurementsStorage).
-
-  honeOne.
-
-  hone
-  match goal with
-  | _:?AbsR _ _
-    |- _ =>
-        match type of AbsR with
-        | UnConstrQueryStructure _ -> ?T -> Prop =>
-            let storages := storageOf T in
-            pose AbsR; pose storages
-        end
-  end.
-
-  startMethod Weather_AbsR. 
-  concretize.
-  asPerm (CellsStorage, MeasurementsStorage).
-
-  Eval cbv delta [CellsStorage] in CellsStorage.
-  Print Ltac fields.
-  
-  Ltac check_for_attr_list X :=
-    match type of X with
-      | list (Attributes _) => idtac
-    end.
-
-  Ltac pull_attributes_list body :=
-    match body with
-      | let x := ?X in _ => check_for_attr_list X; X
-      | let x := ?X in let y := ?Y in _ => check_for_attr_list Y; 
-                                          Y
-      | _ => fail "No list of attributes found"
-    end.
-
-  Unset Ltac Debug.
-  pull_attributes_list ltac:(eval cbv delta [CellsStorage] in CellsStorage).
-
-  let fs := pull_attributes_list CellsStorage in pose (fs' := fs). 
-
-
-  
-  match  with
-    | let src := ?X in ?body => X
-  end
-
-
-  match type of fs' with
-    | ?a => assert a
-  end.
-  compute in fs'.
-
-  
-  unfold WeatherSchema in fs'.
-  Unset Printing Notations. Show. 
-  unfold QSGetNRelSchemaHeading, GetNRelSchemaHeading, schemaHeading, GetNRelSchema in fs'. simpl in fs'. idtac "hello".
-  useIndex CellsStorage.
-
-  Print Ltac concretize1.
-  
-asPerm storages; commit; choose_db AbsR;
-  finish honing.
-observer' AbsR storages
-  (*unfold cast, eq_rect_r, eq_rect, eq_sym.*)
-  Notation "a ! b" := (a ``(b)).
-  Notation "a == b" := (if string_dec a b then true else false).
-  Notation "a != b" := (negb (beq_nat b a)) (at level 20, no associativity).
-  Notation "a == b" := (beq_nat b a).
-  repeat match goal with
-           | [ H := _ |- _ ] => unfold H; clear H
-         end.
+  plan Weather_AbsR.
   finish sharpening.
 Defined.
